0507

plc/Nameless.v
@@ -1,5 +1,6 @@
-From Stdlib Require Import FunctionalExtensionality.
 From Stdlib Require Import Nat.
+From Stdlib Require Import List.
+From Stdlib Require Import FunctionalExtensionality.
 
 From PLC Require Export Maps TyAndTm.
 
@@ -21,7 +22,7 @@ Notation "<{{ T }}>" := T (T custom plc_ty at level 99) : plc_scope.
 (* ----- 型 (ty) の Notation ----- *)
 Notation "( T )" := T (in custom plc_ty, T custom plc_ty at level 99) : plc_scope.
 Notation "T1 -> T2" := (TyArrow T1 T2) (in custom plc_ty at level 50, right associativity) : plc_scope.
-Notation "'-/', T" := (TyForall T) (in custom plc_ty at level 90, T custom plc_ty at level 90) : plc_scope.
+Notation "'-/,' T" := (TyForall T) (in custom plc_ty at level 90, T custom plc_ty at level 90) : plc_scope.
 Notation "'Unit'" := TyUnit (in custom plc_ty at level 0) : plc_scope.
 
 Notation "<{ t }>" := t (t custom plc_tm at level 200) : plc_scope.
@@ -55,7 +56,6 @@ Hint Unfold X : core.
 Hint Unfold Y : core.
 Hint Unfold Z : core.
 
-
 Definition sigma_tm_empty : nat -> vl := fun n => var_vl n.
 Definition sigma_tm_one (x: nat) (s: vl) : nat -> vl :=
   fun n => if n=?x then s else n.
@@ -64,9 +64,9 @@ Definition sigma_ty_one (X: nat) (S: ty) : nat -> ty :=
   fun n => if n=?X then S else n.
 
 Notation "'(' x '\->' s ')'" := (sigma_tm_one x s) (in custom plc_tmsubst).
-Notation "'(' X '\->' S ')'" := (sigma_tm_one X S) (in custom plc_tmsubst).
+Notation "'(' X '\->' S ')'" := (sigma_ty_one X S) (in custom plc_tysubst).
 
-Notation "'[' X ':=' S ']' T" := (subst_ty (sigma_tm_one X S) T)
+Notation "'[' X ':=' S ']' T" := (subst_ty (sigma_ty_one X S) T)
     (in custom plc_ty at level 5, T custom plc_ty at next level, right associativity).
 
 Notation "'[[' x ':=' s ']]' t" := (subst_tm sigma_ty_empty (sigma_tm_one x s) t)
@@ -87,22 +87,39 @@ Notation " 'return' e "
 Notation " 'fail' "
   := None.
 
+Scheme tm_mut_ind := Induction for tm Sort Prop
+with   vl_mut_ind := Induction for vl Sort Prop.
+
+Combined Scheme tm_vl_mut_ind from tm_mut_ind, vl_mut_ind.
+
+Definition beta_red t v := 
+  ren_tm id Nat.pred (
+    subst_tm sigma_ty_empty (sigma_tm_one 0 (ren_vl id S v)) t
+  ).
+
+Definition ty_beta_red t T :=
+  ren_tm Nat.pred id (
+    subst_tm (sigma_ty_one 0 (ren_ty S T)) sigma_tm_empty t
+  ).
+
 Fixpoint eval_tm (t: tm) : option tm :=
   match t with
   | <{ t1 t2 }> =>
       match t1, t2 with
-      | TmVal <{ \:T, t11' }>, TmVal v2 => return <{ [[0:=v2]] t11' }>
-      | TmVal <{ \:T, t11' }>, t2 =>
+      | TmVal <{ \:T, t11' }>, TmVal v2 => 
+          return (beta_red t11' v2)
+      | TmVal _, TmVal _ => fail
+      | TmVal _, t2 =>
           t2' <- eval_tm t2 ;;
           return <{ t1 t2' }>
-      | TmVal _, t2 => fail
       | t1, t2 => 
           t1' <- eval_tm t1 ;;
           return <{ t1' t2 }>
       end
   | <{ t1 [T] }> =>
       match t1 with 
-      | TmVal <{ \\, t11' }> => return <{ [0:=T] t11' }>
+      | TmVal <{ \\, t11' }> =>
+          return (ty_beta_red t11' T)
       | t1 =>
           t1' <- eval_tm t1 ;;
           return <{ t1' [T] }>
@@ -127,3 +144,501 @@ Fixpoint eval_tm_big (t: tm) : option tm :=
       end
   | TmVal _ => return t 
   end.
+
+Definition context := list ty.
+
+Scheme Equality for ty.
+Notation "T1 '=^?' T2" := (ty_beq T1 T2) (at level 70, no associativity).
+
+
+
+Definition typing_beta_red T U := 
+  ren_ty Nat.pred (
+    subst_ty (sigma_ty_one 0 (ren_ty S U)) T
+  ).
+
+Fixpoint typing (Gamma: context) (t: tm) : option ty :=
+  match t with
+  | <{ t1 t2 }> =>
+      T1 <- typing Gamma t1 ;;
+      T2 <- typing Gamma t2 ;;
+      match T1 with
+        | <{{ T11 -> T12 }}> =>
+            if (T11=^?T2) then return T12 else fail
+        | _ => fail
+      end
+  | <{ t1 [T] }> =>
+      T1 <- typing Gamma t1 ;;
+      match T1 with 
+      | <{{ -/, T11 }}> =>
+          return typing_beta_red T11 T
+      | _ => fail
+      end
+  | TmVal v => typing_vl Gamma v
+  end
+with typing_vl (Gamma: context) (v: vl) : option ty := 
+  match v with
+  | var_vl X => List.nth_error Gamma X
+  | <{ \:T, t1 }> =>
+      T1 <- typing (T :: Gamma) t1 ;;
+      return <{{T -> T1}}>
+  | <{ \\, t1 }> => 
+      T1 <- typing (map (ren_ty S) Gamma) t1 ;;
+      return <{{-/, T1}}>
+  | <{ unit }> => return <{{Unit}}>
+  end.
+
+Lemma normal_form_abs : forall v T1 T2,
+  typing nil (TmVal v) = Some <{{T1 -> T2}}> ->
+  exists T t, v = <{ \:T, t }>.
+Proof.
+  intros v T1 T2 H.
+  destruct v; simpl in H; try discriminate.
+  - rewrite nth_error_nil in H. discriminate.
+  - eauto.
+  - destruct (typing nil t); discriminate.
+Qed.
+
+Lemma normal_form_tyabs : forall v T,
+  typing nil (TmVal v) = Some <{{-/, T}}> ->
+  exists t, v = <{ \\, t }>.
+Proof.
+  intros v T H.
+  destruct v; simpl in H; try discriminate.
+  - rewrite nth_error_nil in H. discriminate.
+  - destruct (typing (t :: nil) t0); discriminate.
+  - eauto.
+Qed.
+
+Theorem Progress : forall t T,
+  typing nil t = Some T ->
+  (exists t', eval_tm t = Some t') \/ (exists v, t = TmVal v).
+Proof.
+  induction t; intros.
+  - left. simpl in H.
+    destruct (typing nil t1) as [T1|] eqn: Tyt1;
+    destruct (typing nil t2) as [T2|] eqn: Tyt2;
+    try discriminate.
+    destruct T1 as [|T11 T12| | ] eqn:EqT1; try discriminate.
+    destruct (T11 =^? T2) eqn: EqT2; try discriminate.
+    inversion H.
+    specialize (IHt1 <{{T11->T12}}>) as [ [t1' IHt1']|[v1' IHt1'] ];
+    try reflexivity.
+    + exists <{ t1' t2 }>.
+      simpl. rewrite IHt1'. destruct t1; try reflexivity.
+      simpl in IHt1'. discriminate.
+    + specialize (IHt2 T2) as [ [t2' IHt2']|[v2' IHt2'] ];
+      try reflexivity.
+      * exists <{ t1 t2' }>.
+        simpl. rewrite IHt2'. subst t1.
+        destruct v1' eqn: Ev1'; destruct t2 eqn: Et2;
+        try reflexivity; try discriminate IHt2'.
+      * subst t1 t2. apply normal_form_abs in Tyt1 as [T' [t' Eqt'] ].
+        subst v1'. eexists. reflexivity.
+  - left. simpl in H.
+    destruct (typing nil t) as [T1|] eqn: Tyt; try discriminate.
+    destruct T1 as [| | T11 | ] eqn:EqT1; try discriminate.
+    specialize (IHt <{{-/, T11}}>) as [ [t1' IHt1']|[v1' IHt1'] ];
+    try reflexivity.
+    + eexists. simpl. rewrite IHt1'. destruct t; try reflexivity.
+      simpl in IHt1'. discriminate.
+    + subst t. apply normal_form_tyabs in Tyt as [t' Ht'].
+      subst. eexists. reflexivity.
+  - right. eexists. reflexivity.
+Qed.
+
+Definition shift_tm t := ren_tm id S t.
+Definition shift_ty T := ren_ty S T.
+
+Lemma ty_beq_eq : forall T1 T2,
+  T1 =^? T2 = true <-> T1 = T2.
+Proof.
+  intros T1 T2.
+  split; intro H.
+  - apply internal_ty_dec_bl. assumption.
+  - subst. apply internal_ty_dec_lb. reflexivity.
+Qed.
+
+Lemma ty_beq_refl : 
+forall T, T =^? T = true.
+Proof.
+  intros T. apply ty_beq_eq. reflexivity.
+Qed.
+
+Lemma invert_typing_app : forall Gamma t1 t2 T, 
+  typing Gamma <{ t1 t2 }> = return T ->
+  exists T1, (
+    typing Gamma t1 = return <{{T1 -> T}}> /\
+    typing Gamma t2 = return T1
+  ).
+Proof.
+  intros Gamma t1 t2 T H.
+  simpl in H.
+  destruct (typing Gamma t1) as [T1|] eqn:E1; try discriminate.
+  destruct (typing Gamma t2) as [T2|] eqn:E2; try discriminate.
+  destruct T1 as [|T11 T12| |]; try discriminate.
+  destruct (T11 =^? T2) eqn:E3; try discriminate.
+  apply ty_beq_eq in E3. subst T2.
+  inversion H; subst.
+  eexists; eauto.
+Qed.
+
+Lemma invert_typing_tyapp : forall Gamma t1 S T, 
+  typing Gamma <{ t1 [S] }> = return T ->
+  exists T1, (
+    typing Gamma t1 = return <{{ -/, T1 }}> /\
+    T = typing_beta_red T1 S
+  ).
+Proof.
+  intros Gamma t S T H.
+  simpl in H.
+  destruct (typing Gamma t) as [T1'|] eqn:Eq; try discriminate.
+  destruct T1' as [| | T11 |]; try discriminate.
+  inversion H; subst.
+  eexists. split; reflexivity.
+Qed.
+
+Lemma weaking_var :
+  (
+    forall t Gamma T,
+    typing Gamma t = Some T ->
+    forall Delta xi,
+    (forall x U, nth_error Gamma x = Some U -> 
+                nth_error Delta (xi x) = Some U) ->
+    typing Delta (ren_tm id xi t) = Some T
+  ) /\ (
+    forall v Gamma T,
+    typing_vl Gamma v = Some T ->
+    forall Delta xi,
+    (forall x U, nth_error Gamma x = Some U -> 
+                  nth_error Delta (xi x) = Some U) ->
+    typing_vl Delta (ren_vl id xi v) = Some T
+  ).
+Proof.
+  apply tm_vl_mut_ind; intros.
+  - simpl. rename H into IHt1. rename H0 into IHt2.
+    specialize (invert_typing_app _ _ _ _ H1) as [T1 [Ht1 Ht2] ].
+    rewrite IHt1 with (T:=<{{ T1 -> T }}>) (Gamma:=Gamma);
+    try assumption.
+    rewrite IHt2 with (T:=T1) (Gamma:=Gamma); try assumption.
+    rewrite ty_beq_refl. reflexivity.
+  - simpl. rename H into IHt.
+    specialize (invert_typing_tyapp _ _ _ _ H0) as [T1 [Ht1 HT] ].
+    rewrite IHt with (T:=<{{ -/, T1 }}>) (Gamma:=Gamma); try assumption.
+    replace (ren_ty id t0) with t0 by (symmetry; apply rinstId'_ty).
+    f_equal. symmetry. assumption.
+  - destruct v; simpl; simpl in H; simpl in H0.
+    + apply H1. assumption.
+    + replace (ren_ty id t) with t by (symmetry; apply rinstId'_ty).
+      simpl. replace (ren_ty id t) with t in H by (symmetry; apply rinstId'_ty) .
+      apply H with (Gamma:=Gamma); assumption.
+    + apply H with (Gamma:=Gamma); assumption.
+    + assumption.
+  - simpl in *. apply H0. assumption.
+  - simpl in *.
+    replace (ren_ty id t) with t by (symmetry; apply rinstId'_ty).
+    destruct (typing (t :: Gamma) t0) eqn: Tyt; try discriminate.
+    inversion H0.
+    assert (Ht: 
+      typing (t::Delta) (ren_tm (upRen_vl_ty id) (upRen_vl_vl xi) t0) = return t1
+    ).
+    { replace (upRen_vl_ty id) with (@id nat) by (unfold upRen_vl_ty; reflexivity).
+      apply H with (Gamma:=(t::Gamma)); try assumption. 
+      intros. destruct x0; simpl in *.
+      - assumption.
+      - apply H1. assumption. }
+    rewrite Ht. reflexivity.
+  - simpl in *.
+    replace (upRen_ty_ty id) with (@id nat) by
+    ( unfold upRen_ty_ty; unfold unscoped.up_ren;
+      apply functional_extensionality; destruct x0; reflexivity).
+    destruct (typing (map (ren_ty S) Gamma) t) eqn: Tyt; try discriminate.
+    inversion H0.
+    assert (Ht:
+      typing (map (ren_ty S) Delta) (ren_tm id (upRen_ty_vl xi) t) = return t0
+    ).
+    { apply H with (map (ren_ty S) Gamma); try assumption.
+      intros. unfold upRen_ty_vl.
+      rewrite nth_error_map in *.
+      destruct (nth_error Gamma x0) eqn: NthG.
+      - rewrite H1 with (U:=t1); assumption.
+      - discriminate H2. }
+    rewrite Ht. reflexivity.
+  - simpl in *. assumption.
+Qed.
+
+Lemma sigma_ty_empty_stable : forall T,
+  T = subst_ty sigma_ty_empty T.
+Proof.
+  intros T. unfold sigma_ty_empty. symmetry. apply idSubst_ty.
+  reflexivity.
+Qed.
+
+Lemma typingbeta_ren_commutable : forall T U xi,
+  typing_beta_red (ren_ty (upRen_ty_ty xi) T) (ren_ty xi U) =
+  ren_ty xi (typing_beta_red T U).
+Proof.
+  induction T; intros;
+  unfold typing_beta_red, sigma_ty_one in *.
+  - simpl in *. destruct n as [|n'] eqn: Eqn'.
+    + simpl. repeat rewrite (renRen_ty S pred).
+      unfold core.funcomp. simpl. repeat rewrite rinstId'_ty.
+      reflexivity.
+    + reflexivity.
+  - simpl in *. rewrite IHT1. rewrite IHT2. reflexivity.
+  - simpl. Search up_ty_ty. admit.
+  - reflexivity.
+Admitted.  
+
+Lemma weaking_tyvar :
+  (
+    forall t Gamma T,
+    typing Gamma t = Some T ->
+    forall Delta xi,
+    (forall x U, nth_error Gamma x = Some U -> 
+                 nth_error Delta x = Some (ren_ty xi U)) ->
+    typing Delta (ren_tm xi id t) = Some (ren_ty xi T)
+  ) /\ (
+    forall v Gamma T,
+    typing_vl Gamma v = Some T ->
+    forall Delta xi,
+    (forall x U, nth_error Gamma x = Some U -> 
+                 nth_error Delta x = Some (ren_ty xi U)) ->
+    typing_vl Delta (ren_vl xi id v) = Some (ren_ty xi T)
+  ).
+Proof.
+  apply tm_vl_mut_ind; intros; simpl.
+  - rename t into t1, t0 into t2, H into IH1, H0 into IH2.
+    apply invert_typing_app in H1 as [T1 [Tyt1 Tyt2] ].
+    rewrite IH1 with (Gamma:=Gamma) (T:=<{{T1->T}}>); try assumption.
+    rewrite IH2 with (Gamma:=Gamma) (T:=T1); try assumption.
+    cbn [ren_ty]. rewrite ty_beq_refl. reflexivity.
+  - apply invert_typing_tyapp in H0 as [T1 [Tyt EqT] ].
+    rewrite H with (Gamma:=Gamma) (T:=<{{ -/, T1}}>); try assumption.
+    cbn [ren_ty]. subst T.
+    
+    rewrite typingbeta_ren_commutable.
+    reflexivity.
+  - 
+  
+Admitted.
+  
+
+Lemma context_shift : forall Gamma x sigma T,
+  typing_vl Gamma (sigma x) = return T ->
+  typing_vl (map (ren_ty S) Gamma) (up_ty_vl sigma x) = return ren_ty S T.
+Proof.
+  intros. unfold up_ty_vl, core.funcomp, unscoped.shift, unscoped.id.
+  apply weaking_tyvar with (Gamma:=Gamma).
+  - apply H.
+  - intros x' U Hnth.
+    rewrite nth_error_map.
+    rewrite Hnth. reflexivity.
+Qed.
+
+Theorem var_subst_preserves_typing :
+  (
+    forall t Gamma T,
+    typing Gamma t = Some T ->
+    forall Delta sigma,
+    (forall x U, nth_error Gamma x = Some U -> typing_vl Delta (sigma x) = Some U) ->
+    typing Delta (subst_tm id sigma t) = Some T
+  ) /\ (
+    forall v Gamma T,
+    typing_vl Gamma v = Some T ->
+    forall Delta sigma,
+    (forall x U, nth_error Gamma x = Some U -> typing_vl Delta (sigma x) = Some U) ->
+    typing_vl Delta (subst_vl id sigma v) = Some T
+  ).
+Proof.
+  apply tm_vl_mut_ind; intros.
+  - (* TmApp *)
+    simpl in *.
+    destruct (typing Gamma t) as [T1|] eqn:E1; try discriminate.
+    destruct (typing Gamma t0) as [T2|] eqn:E2; try discriminate.
+    destruct T1 as [|T11 T12| |]; try discriminate.
+    destruct (T11 =^? T2) eqn:E3; try discriminate.
+    inversion H1; subst.
+    simpl.
+    rewrite H with (Delta:=Delta) (sigma:=sigma) (Gamma:=Gamma) (T:=<{{T11->T}}>); auto.
+    rewrite H0 with (Delta:=Delta) (sigma:=sigma) (Gamma:=Gamma) (T:=T2); auto.
+    rewrite E3. reflexivity.
+  - (* TmTApp *)
+    simpl in *.
+    destruct (typing Gamma t) as [T1|] eqn:E1; try discriminate.
+    destruct T1 as [| | T11 |]; try discriminate.
+    inversion H0; subst.
+    simpl.
+    rewrite H with (Delta:=Delta) (sigma:=sigma) (Gamma:=Gamma) (T:=<{{-/,T11}}>); auto.
+    replace (subst_ty (fun x0 : nat => id x0) t0) with t0; try reflexivity.
+    rewrite instId'_ty. reflexivity.
+  - (* TmVal *)
+    simpl in *.
+    apply H with Gamma; auto.
+  - (* var_vl *)
+    simpl in *.
+    apply H0. assumption.
+  - (* TmAbs *)
+    simpl in *.
+    destruct (typing (t :: Gamma) t0) as [T1|] eqn:E1; try discriminate.
+    inversion H0; subst.
+    rewrite H with (Gamma:=(t::Gamma)) (T:=T1).
+    + rewrite instId'_ty. reflexivity.
+    + assumption.
+    + intros. rewrite instId'_ty.
+      destruct x0 as [|x0']; simpl; simpl in H2.
+      * assumption.
+      * unfold core.funcomp, unscoped.shift, unscoped.id.
+        apply weaking_var with (Gamma:=Delta); auto.
+  - (* TmTAbs *)
+    simpl in *.
+    destruct (typing (map (ren_ty S) Gamma) t) as [T1|] eqn:E1; try discriminate.
+    inversion H0; subst.
+    assert (subst_tm (up_ty_ty (fun x0 : nat => id x0)) (up_ty_vl sigma) t
+    = subst_tm (fun x : nat =>  x) (up_ty_vl sigma) t).
+    { apply ext_tm; try reflexivity.
+      intros. destruct x0; reflexivity. }
+    rewrite H2. rewrite (H _ _ E1); try reflexivity.
+    intros. rewrite nth_error_map in H3.
+    destruct (nth_error Gamma x0) as [U' |] eqn: EqU'; try discriminate.
+    simpl in H3. inversion H3. subst U. apply H1 in EqU'.
+    apply context_shift. assumption.
+  - (* TmUnit *)
+    simpl in *.
+    inversion H; subst; reflexivity.
+Qed.
+
+
+
+
+Theorem var_subst_preserves_typing :
+  (
+    forall t Gamma s T S,
+    typing (S :: Gamma) t = return T ->
+    typing_vl Gamma s = return S ->
+    typing Gamma (beta_red t s) = return T
+  ) /\ (
+    forall v Gamma s T S,
+      typing_vl (S :: Gamma) v = return T ->
+      typing_vl Gamma s = return S ->
+      typing Gamma (beta_red (TmVal v) s) = return T
+  ).
+Proof.
+  apply tm_vl_mut_ind; intros.
+  - simpl; unfold beta_red in *.
+    rename H into IHt1. rename H0 into IHt2.
+    apply invert_typing_app in H1 as [T1 [Ht1 Ht2] ].
+    rewrite IHt1 with (T:=<{{T1->T}}>) (S:=S); try assumption.
+    rewrite IHt2 with (T:=T1) (S:=S); try assumption.
+    rewrite ty_beq_refl. reflexivity.
+  - simpl; unfold beta_red in *. rename H into IH.
+    apply invert_typing_tyapp in H0 as [T1 [Ht HT] ].
+    rewrite IH with (T:=<{{-/,T1}}>) (S:=S); try assumption.
+    replace (subst_ty sigma_ty_empty t0) with t0.
+    + subst T. rewrite rinstId'_ty. reflexivity.
+    + apply sigma_ty_empty_stable.
+  - simpl; unfold beta_red in *. rename H into IH.
+    simpl in IH. rewrite IH with (T:=T) (S:=S); auto.
+  - simpl; unfold beta_red in *. unfold sigma_tm_one.
+    destruct n as [|n'] eqn: Eqn; simpl; simpl in H0.
+    + rewrite renRen_vl. unfold core.funcomp, id.
+      simpl. rewrite rinstId'_vl.
+      simpl in H. rewrite H0. assumption.
+    + simpl in H. assumption.
+  - simpl. simpl in H0. rewrite instId'_ty. rewrite rinstId'_ty.
+    destruct (typing (t::S::Gamma) t0) as [T1|] eqn: Tyt0; try discriminate.
+    inversion H0. 
+    replace (upRen_vl_ty id) with (@id nat) by (unfold upRen_vl_ty; reflexivity).
+    replace (up_vl_ty sigma_ty_empty) with sigma_ty_empty by (unfold up_vl_ty; reflexivity).
+    unfold beta_red in H.
+    replace (upRen_vl_vl pred) with (@id nat).
+    + admit.
+    + apply functional_extensionality. intros.
+      unfold upRen_vl_vl, unscoped.up_ren, unscoped.scons. destruct x0.
+      * reflexivity.
+      * simpl. unfold core.funcomp. 
+    unfold up_vl_vl, unscoped.scons, unscoped.var_zero,
+    unscoped.id, unscoped.shift, core.funcomp.
+    simpl in H. admit.
+  - simpl; unfold beta_red in *.
+    replace (upRen_ty_ty id) with (@id nat) by (apply functional_extensionality; intros; destruct x0; reflexivity).
+    replace (up_ty_ty sigma_ty_empty) with sigma_ty_empty by (apply functional_extensionality; intros; destruct x0; reflexivity).
+    simpl in H0.
+    destruct (typing (ren_ty Datatypes.S S :: map (ren_ty Datatypes.S) Gamma) t) as [T1|] eqn: Tyt1;
+    inversion H0.
+    apply H with (s:=s) in Tyt1.
+    + replace (upRen_ty_vl pred) with pred
+      by (apply functional_extensionality; intros; destruct x0; reflexivity).
+      replace (up_ty_vl (sigma_tm_one 0 (ren_vl id Datatypes.S s))) with (sigma_tm_one 0 (ren_vl id Datatypes.S s)).
+      rewrite Tyt1. reflexivity.
+      * admit.
+    + admit.
+    
+
+    rewrite weaking_var with (Gamma:=(S::t::Gamma)) (T:=T1).
+    + reflexivity.
+    + admit.
+    + intros. destruct x0 as [|x0'].
+      * simpl; simpl in H2.  assumption.
+      * simpl. simpl in H2.  destruct x0'.
+        { simpl in H2. simpl. admit.    }
+        { simpl in H2. simpl. assumption. }
+    
+    Search subst_tm.
+    + simpl in IH.
+      rewrite IH with (T:=T) (S:=S); auto.
+    + simpl in IH.
+      rewrite IH with (T:=T) (S:=S); auto.
+    + assumption.
+  - 
+   
+Admitted.
+
+
+Theorem Preservation : forall Gamma t t' T,
+  typing Gamma t = Some T ->
+  eval_tm t = Some t' ->
+  typing Gamma t' = Some T.
+Proof.
+  intros Gamma t. generalize dependent Gamma.
+  induction t; intros Gamma t' T Hty Heval.
+  - apply invert_typing_app in Hty as [T1 [Hty1 Hty2] ].
+    simpl in Heval. destruct t1 eqn: Eqt1;
+    try (
+      rewrite <- Eqt1 in *;
+      destruct (eval_tm t1) as [t1' |] eqn: evt1';
+      inversion Heval;
+      simpl; rewrite IHt1 with (T:=<{{T1->T}}>); auto;
+      rewrite Hty2; rewrite ty_beq_refl; reflexivity
+    ).
+    + destruct (eval_tm t2) as [t2' |] eqn: evt2'.
+      * destruct t2 eqn: Eqt2; 
+        try (
+          rewrite <- Eqt2 in *;
+          destruct v eqn: Eqv; rewrite <- Eqv in *; inversion Heval;
+          simpl; simpl in Hty1; rewrite Hty1;
+          apply IHt2 with (t':=t2') in Hty2; try reflexivity;
+          rewrite Hty2; rewrite ty_beq_refl; reflexivity
+        ).
+        discriminate.
+      * destruct v; destruct t2; try discriminate.
+        inversion Heval. simpl in Hty2.
+        simpl in Hty1. destruct (typing (t :: Gamma) t0) eqn: Tyt0;
+        try discriminate. inversion Hty1. subst t t2.
+        apply var_subst_preserves_typing with T1; assumption.
+  - rename t into t1.
+    apply invert_typing_tyapp in Hty as [T1 [Hty HT] ].
+    simpl in Heval.
+    destruct (eval_tm t1) as [t1' |] eqn: evt1'.
+    + destruct t1 eqn: Eqt1;
+      try (
+        rewrite <- Eqt1 in *; inversion Heval;
+        simpl; rewrite IHt with (T:=<{{-/, T1}}>); auto;
+        subst T; reflexivity
+      ).
+      simpl in evt1'. discriminate.
+    + destruct t1 eqn: Eqt1; try destruct v; try discriminate.
+      admit.
+  - discriminate.
+Admitted.
+
